\section{Cubic Spline Interpolation}
\begin{defn}
Given a function $f$ defined on $[a,b]$, $a=x_0<x_1<\cdots,<x_n=b$, a cubic spline interpolation $S$ for $f$ is a function that satisfies the following conditions.
\begin{enumerate}
    \item $S_j(x)$ is a cubic polynomial, on the subinterval $[x_j,x_{j+1}]$ for $j=0:n-1$.
    \item $S_j(x_j)=f(x_j)$, $S_j(x_{j+1})=f(x_{j+1})$ for $j=0:n-2$.
    \item $S'_j(x_{j+1})=S'_{j+1}(x_{j+1})$ for $j=0:n-2$.
    \item $S''_j(x_{j+1})=S''_{j+1}(x_{j+1})$ for $j=0:n-2$.
    \item $\begin{cases}
          \text{natural boundary:} & S''(x_0)=S''(x_n)=0. \\
          \text{clamped boundary:} & S'(x_0)=f'(x_0)$, $S'(x_n)=f'(x_n).
          \end{cases}$
\end{enumerate}
\end{defn}
\subsection{Construction of a Cubic Spline}
Let $h_j=x_{j+1}-x_j$ (forward):
\begin{enumerate}[(1)]
    \item \begin{align*}
          S_j(x) &= a_j+b_j(x-x_j)+c_j(x-x_j)^2+d_j(x-x_j)^3\quad\text{for $j=0:n-1$} \\
          &\Rightarrow a_{j+1}=S_{j+1}(x_{j+1})=S_j(x_{j+1}) \\
          &\hspace{1.3cm}=a_j+b_jh_j+c_jh_j^2+d_jh_j^3=f(x_{j+1})\quad\text{for $j=0:n-1$}
          \end{align*}
    \item \begin{align*}
          S'_j(x) &= b_j+2c_j(x-x_j)+3d_j(x-x_j)^2 \\
          &\Rightarrow b_{j+1}=S'_{j+1}(x_{j+1})=S'_j(x_{j+1}) \\
          &\hspace{1.3cm}=b_j+2c_jh_j+3d_jh_j^2\quad\text{for $j=0:n-1$}
          \end{align*}
    \item \begin{align*}
          S''_j(x) &= 2c_j+6d_j(x-x_j) \\
          &\Rightarrow 2c_{j+1}=S''_{j+1}(x_{j+1})=S''_j(x_{j+1}) \\
          &\hspace{1.3cm}=2c_j+6d_jh_j\quad\text{for $j=0:n-1$}
          \end{align*}
\end{enumerate}

Above all, the linear system to be solved is:
\begin{align*}
    &Ax=b \\
    &\begin{cases}
    A=diag([1,2(h_0+h_1),\cdots,2(h_{n-2}+h_{n-1}),1]) \\
    \phantom{A=}+diag([0,h_1,\cdots,h_{n-1}],1)+diag([h_0,\cdots,h_{n-2},0],-1) \\
    x = [c_0;c_1;\cdots;c_n] \\
    b = \left[0;\frac{3}{h_1}(a_2-a_1)-\frac{3}{h_0}(a_1-a_0);\cdots;\frac{3}{h_{n-1}}(a_n-a_{n-1})-\frac{3}{h_{n-2}}(a_{n-1}-a_{n-2});0\right] \\
    \end{cases}
\end{align*}
Then we will get $b_j$, $d_j$ by
\begin{equation*}
    \begin{cases}
    b_j &= \frac{1}{h_j}(a_{j+1}-a_j)-\frac{h_j}{3}(2c_j+c_{j+1}) \\
    d_j &= \frac{1}{3h_j}(c_{j+1}-c_j)
    \end{cases}
\end{equation*}

\subsection{Clamped Splines}
\begin{align*}
    &Ax=b \\
    &\begin{cases}
    A=\begin{pmatrix}
      2h_0 & h_0 & 0 & \cdots & 0 \\
      h_0 & 2(h_0+h_1) & h_1 & \ddots & \vdots \\
      0 & h_1 & 2(h_1+h_2) & \ddots & \vdots \\
      \vdots & \ddots & \ddots & \ddots & h_{n-1} \\
      0 & \cdots & \cdots & h_{n-1} & 2h_{n-1} \\
      \end{pmatrix} \\
    \\
    x = \begin{pmatrix}c_0 & c_1 & \cdots & c_n \end{pmatrix}^T \\
    \\
    b = \begin{pmatrix}
        \frac{3}{h_0}(a_1-a_0)-3f'(a) \\
        \frac{3}{h_1}(a_2-a_1)-\frac{3}{h_0}(a_1-a_0) \\
        \vdots \\
        \frac{3}{h_{n-1}}(a_n-a_{n-1})-\frac{3}{h_{n-2}}(a_{n-1}-a_{n-2}) \\
        3f'(b)-\frac{3}{h_{n-1}}(a_n-a_{n-1})
        \end{pmatrix}
    \end{cases}
\end{align*}