\section{Linear Systems of Equations and Pivoting Strategies}
\subsection{Gaussian Elimination with Backward Substitution}
\begin{align*}
    E1: & a_{11}x_{1}+a{12}x_{2}+\cdots+a_{1n}x_{n} = a_{1,n+1} \\
    E2: & a_{21}x_{1}+a{22}x_{2}+\cdots+a_{2n}x_{n} = a_{2,n+1} \\
    & \vdots \\
    En: & a_{n1}x_{1}+a{n2}x_{2}+\cdots+a_{nn}x_{n} = a_{n,n+1} \\
\end{align*}

\subsection{Operation Counts}
\subsubsection{Multiplications / divisions}
\[
\sum_{i=1}^{n-1}(n-i)+(n-i)(n-i+1)=\frac{2n^3+3n^2-5n}{6}
\]
\subsubsection{Additions / subtractions}
\[
\sum_{i=1}^{n-1}(n-i)(n-i+1)=\frac{n^3-n}{3}
\]
\subsection{Backward substitution *\&/}
\[
1+\sum_{i=1}^{n-1}((n-i)+1)=\frac{n^2+n}{2}
\]
\subsection{Backward substitution +\&-}
\[
\sum_{i=1}^{n-1}((n-i-1)+1)=\frac{n^2-n}{2}
\]

\subsection{Gaussian Elimination with Partial Pivoting}
\begin{python}
def gaussian_elimination_partial_pivoting(A, b):
    np_result = A**-1 * b
    print(np_result.T)
    n = A.shape[0]
    x = np.zeros((n,1))
    tmp = 0
    for k in range(n-1):
        M = k
        for m in range(k+1,n):
            if A[m,k] > A[M,k]: M = m
        A[[k,M]] = A[[M,k]]
        b[[k,M]] = b[[M,k]]
        for i in range(k+1,n):
            m = A[i,k] / A[k,k]
            for j in range(k,n):
                A[i,j] = A[i,j] - m*A[k,j]
            b[i,0] = b[i,0] - m*b[k,0]
    x[-1,0] = b[-1,0] / A[-1,-1]
    for i in range(n-2,-1,-1):
        for j in range(i+1,n):
            tmp += A[i,j] * x[j,0]
        x[i,0] = (b[i,0] - tmp) / A[i,i]
        tmp = 0
    return x
\end{python}

\subsection{Gaussian Elimination with Scaled Partial Pivoting}
\begin{python}
def gaussian_elimination_scaled_partial_pivoting(A, b):
    np_result = A**-1 * b
    print(np_result.T)
    n = A.shape[0]
    x = np.zeros((n,1))
    tmp = 0
    for k in range(n):
        M = np.max(A[k,:])
        A[k,:] /= M
        b[k,0] /= M
    for k in range(n-1):
        for i in range(k+1,n):
            m = A[i,k] / A[k,k]
            for j in range(k,n):
                A[i,j] = A[i,j] - m*A[k,j]
            b[i,0] = b[i,0] - m*b[k,0]
    x[-1,0] = b[-1,0] / A[-1,-1]
    for i in range(n-2,-1,-1):
        for j in range(i+1,n):
            tmp += A[i,j] * x[j,0]
        x[i,0] = (b[i,0] - tmp) / A[i,i]
        tmp = 0
    return x
\end{python}